theories/std/inf_array.v
@@ -16,129 +16,142 @@ Record inf_array `{!heapGS Σ} {unboxed : bool} := {
   inf_array_get : val ;
   inf_array_set : val ;
 
-  inf_array_model : val → (nat → val) → iProp Σ ;
+  inf_array_name : Type ;
+  inf_array_name_eq_dec :
+    EqDecision inf_array_name ;
+  inf_array_name_countable :
+    Countable inf_array_name ;
 
-  inf_array_model_timeless t vs :
-    Timeless (inf_array_model t vs) ;
+  inf_array_inv : val → inf_array_name → namespace → iProp Σ ;
+  inf_array_model : val → inf_array_name → (nat → val) → iProp Σ ;
 
-  inf_array_make_spec v :
+  inf_array_inv_persistent t γ ι :
+    Persistent (inf_array_inv t γ ι) ;
+  inf_array_model_timeless t γ vs :
+    Timeless (inf_array_model t γ vs) ;
+
+  inf_array_make_spec ι v :
     {{{ True }}}
       inf_array_make v
-    {{{ t,
+    {{{ t γ,
       RET t;
-      inf_array_model t (λ _, v)
+      inf_array_inv t γ ι ∗
+      inf_array_model t γ (λ _, v)
     }}} ;
 
-  inf_array_get_spec t i :
+  inf_array_get_spec t γ i ι :
     (0 ≤ i)%Z →
     <<<
-      True
-    | ∀∀ vs, inf_array_model t vs
+      inf_array_inv t γ ι
+    | ∀∀ vs, inf_array_model t γ vs
     >>>
-      inf_array_get t #i
+      inf_array_get t #i @ ↑ι
     <<<
-      inf_array_model t vs
+      inf_array_model t γ vs
     | RET vs (Z.to_nat i); True
     >>> ;
 
-  inf_array_set_spec t i v :
+  inf_array_set_spec t γ ι i v :
     (0 ≤ i)%Z →
     <<<
-      True
-    | ∀∀ vs, inf_array_model t vs
+      inf_array_inv t γ ι
+    | ∀∀ vs, inf_array_model t γ vs
     >>>
-      inf_array_set t #i v
+      inf_array_set t #i v @ ↑ι
     <<<
-      inf_array_model t (<[Z.to_nat i := v]> vs)
+      inf_array_model t γ (<[Z.to_nat i := v]> vs)
     | RET #(); True
     >>> ;
 
   inf_array_unboxed :
-    if unboxed then ∀ t vs,
-      inf_array_model t vs -∗
+    if unboxed then ∀ t γ ι,
+      inf_array_inv t γ ι -∗
       ⌜val_is_unboxed t⌝
     else
       True ;
 }.
 #[global] Arguments inf_array _ {_} _ : assert.
-#[global] Arguments Build_inf_array {_ _} _ {_ _ _ _ _} _ _ _ _ : assert.
+#[global] Arguments Build_inf_array {_ _} _ {_ _ _ _ _ _ _ _ _ _} _ _ _ _ : assert.
+#[global] Existing Instance inf_array_name_eq_dec.
+#[global] Existing Instance inf_array_name_countable.
+#[global] Existing Instance inf_array_inv_persistent.
 #[global] Existing Instance inf_array_model_timeless.
 
 Section inf_array.
   Context `{!heapGS Σ} {unboxed} (inf_array : inf_array Σ unboxed).
 
-  #[global] Instance inf_array_model_ne t n :
-    Proper (pointwise_relation nat (=) ==> (≡{n}≡)) (inf_array.(inf_array_model) t).
+  #[global] Instance inf_array_model_ne t γ n :
+    Proper (pointwise_relation nat (=) ==> (≡{n}≡)) (inf_array.(inf_array_model) t γ).
   Proof.
     intros vs1 vs2 ->%functional_extensionality. done.
   Qed.
-  #[global] Instance inf_array_model_proper t :
-    Proper (pointwise_relation nat (=) ==> (≡)) (inf_array.(inf_array_model) t).
+  #[global] Instance inf_array_model_proper t γ :
+    Proper (pointwise_relation nat (=) ==> (≡)) (inf_array.(inf_array_model) t γ).
   Proof.
     intros vs1 vs2 Hvs. rewrite equiv_dist. solve_proper.
   Qed.
 
-  Definition inf_array_model' t vsₗ vsᵣ :=
-    inf_array.(inf_array_model) t (
+  Definition inf_array_model' t γ vsₗ vsᵣ :=
+    inf_array.(inf_array_model) t γ (
       λ i,
         if decide (i < length vsₗ) then vsₗ !!! i else vsᵣ (i - length vsₗ)
     ).
 
-  #[global] Instance inf_array_model'_ne t n :
-    Proper ((=) ==> pointwise_relation nat (=) ==> (≡{n}≡)) (inf_array_model' t).
+  #[global] Instance inf_array_model'_ne t γ n :
+    Proper ((=) ==> pointwise_relation nat (=) ==> (≡{n}≡)) (inf_array_model' t γ).
   Proof.
     solve_proper.
   Qed.
-  #[global] Instance inf_array_model'_proper t :
-    Proper ((=) ==> pointwise_relation nat (=) ==> (≡)) (inf_array_model' t).
+  #[global] Instance inf_array_model'_proper t γ :
+    Proper ((=) ==> pointwise_relation nat (=) ==> (≡)) (inf_array_model' t γ).
   Proof.
     solve_proper.
   Qed.
-  #[global] Instance inf_array_model'_timeless t vsₗ vsᵣ :
-    Timeless (inf_array_model' t vsₗ vsᵣ).
+  #[global] Instance inf_array_model'_timeless t γ vsₗ vsᵣ :
+    Timeless (inf_array_model' t γ vsₗ vsᵣ).
   Proof.
     apply _.
   Qed.
 
-  Lemma inf_array_get_spec' i t :
+  Lemma inf_array_get_spec' t γ ι i :
     (0 ≤ i)%Z →
     <<<
-      True
-    | ∀∀ vsₗ vsᵣ, inf_array_model' t vsₗ vsᵣ
+      inf_array.(inf_array_inv) t γ ι
+    | ∀∀ vsₗ vsᵣ, inf_array_model' t γ vsₗ vsᵣ
     >>>
-      inf_array.(inf_array_get) t #i
+      inf_array.(inf_array_get) t #i @ ↑ι
     <<<
-      inf_array_model' t vsₗ vsᵣ
+      inf_array_model' t γ vsₗ vsᵣ
     | RET
         let i := Z.to_nat i in
         if decide (i < length vsₗ) then vsₗ !!! i else vsᵣ (i - length vsₗ);
       True
     >>>.
   Proof.
-    iIntros "% !> %Φ _ HΦ".
-    awp_apply (inf_array_get_spec with "[//]"); first done.
+    iIntros "% !> %Φ Hinv HΦ".
+    awp_apply (inf_array_get_spec with "Hinv"); first done.
     iApply (aacc_aupd_commit with "HΦ"); first done.
     iIntros "%vsₗ %vsᵣ Hmodel". iAaccIntro with "Hmodel"; first auto with iFrame.
     iIntros "$ !>". iIntros "HΦ !> _". iApply ("HΦ" with "[//]").
   Qed.
 
-  Lemma inf_array_set_spec' i v t :
+  Lemma inf_array_set_spec' t γ ι i v :
     (0 ≤ i)%Z →
     <<<
-      True
-    | ∀∀ vsₗ vsᵣ, inf_array_model' t vsₗ vsᵣ
+      inf_array.(inf_array_inv) t γ ι
+    | ∀∀ vsₗ vsᵣ, inf_array_model' t γ vsₗ vsᵣ
     >>>
-      inf_array.(inf_array_set) t #i v
+      inf_array.(inf_array_set) t #i v @ ↑ι
     <<<
       let i := Z.to_nat i in
       if decide (i < length vsₗ)
-      then inf_array_model' t (<[i := v]> vsₗ) vsᵣ
-      else inf_array_model' t vsₗ (<[i - length vsₗ := v]> vsᵣ)
+      then inf_array_model' t γ (<[i := v]> vsₗ) vsᵣ
+      else inf_array_model' t γ vsₗ (<[i - length vsₗ := v]> vsᵣ)
     | RET #(); True
     >>>.
   Proof.
-    iIntros "% !> %Φ _ HΦ".
-    awp_apply (inf_array_set_spec with "[//]"); first done.
+    iIntros "% !> %Φ Hinv HΦ".
+    awp_apply (inf_array_set_spec with "Hinv"); first done.
     iApply (aacc_aupd_commit with "HΦ"); first done.
     iIntros "%vsₗ %vsᵣ Hmodel". iAaccIntro with "Hmodel"; first auto with iFrame.
     iIntros "Hmodel !>". iSplitL "Hmodel".
@@ -160,9 +173,9 @@ Section inf_array.
     - iIntros "HΦ !> _". iApply ("HΦ" with "[//]").
   Qed.
 
-  Lemma inf_array_model'_shift t vsₗ v vsᵣ :
-    inf_array_model' t (vsₗ ++ [v]) vsᵣ ⊣⊢
-    inf_array_model' t vsₗ (λ i, match i with 0 => v | S i => vsᵣ i end).
+  Lemma inf_array_model'_shift t γ vsₗ v vsᵣ :
+    inf_array_model' t γ (vsₗ ++ [v]) vsᵣ ⊣⊢
+    inf_array_model' t γ vsₗ (λ i, match i with 0 => v | S i => vsᵣ i end).
   Proof.
     rewrite /inf_array_model' inf_array_model_proper; first done.
     intros j. rewrite app_length /=.
@@ -176,16 +189,16 @@ Section inf_array.
     - rewrite !decide_False; try lia.
       case_match; [lia | f_equal; lia].
   Qed.
-  Lemma inf_array_model'_shift_r t vsₗ v vsᵣ :
-    inf_array_model' t (vsₗ ++ [v]) vsᵣ -∗
-    inf_array_model' t vsₗ (λ i, match i with 0 => v | S i => vsᵣ i end).
+  Lemma inf_array_model'_shift_r t γ vsₗ v vsᵣ :
+    inf_array_model' t γ (vsₗ ++ [v]) vsᵣ -∗
+    inf_array_model' t γ vsₗ (λ i, match i with 0 => v | S i => vsᵣ i end).
   Proof.
     rewrite inf_array_model'_shift //.
   Qed.
-  Lemma inf_array_model'_shift_l t vsₗ vsᵣ v vsᵣ' :
+  Lemma inf_array_model'_shift_l t γ vsₗ vsᵣ v vsᵣ' :
     (∀ i, vsᵣ i = match i with 0 => v | S i => vsᵣ' i end) →
-    inf_array_model' t vsₗ vsᵣ -∗
-    inf_array_model' t (vsₗ ++ [v]) vsᵣ'.
+    inf_array_model' t γ vsₗ vsᵣ -∗
+    inf_array_model' t γ (vsₗ ++ [v]) vsᵣ'.
   Proof.
     intros. rewrite inf_array_model'_shift inf_array_model'_proper //.
   Qed.
